concurrency/aging_lemmas.v
@@ -1,0 +1,300 @@
+Require Import msl.Coqlib2.
+Require Import msl.eq_dec.
+Require Import msl.seplog.
+Require Import veric.juicy_mem.
+Require Import veric.semax_prog.
+Require Import veric.compcert_rmaps.
+Require Import veric.Clight_new.
+Require Import veric.semax.
+Require Import veric.semax_ext.
+Require Import veric.juicy_extspec.
+Require Import veric.tycontext.
+Require Import veric.res_predicates.
+Require Import veric.mem_lessdef.
+Require Import sepcomp.semantics.
+Require Import concurrency.age_to.
+
+Set Bullet Behavior "Strict Subproofs".
+
+Lemma pred_hered {A} {_ : ageable A} (P : pred A) : hereditary age (app_pred P).
+Proof.
+  destruct P; auto.
+Qed.
+
+Ltac hered :=
+  match goal with
+    H : ?P ?x |- ?P ?y => revert H
+  end;
+  match goal with
+    |- ?P ?x -> ?P ?y =>
+    cut (hereditary age P);
+    [ let h := fresh "h" in intros h; apply h; auto | ]
+  end.
+
+Ltac agejoinhyp :=
+  match goal with
+    H : sepalg.join _ _ ?m, A : age ?m _ |- _ =>
+    pose proof age1_join2 _ H A; clear H
+  end.
+
+Ltac agehyps :=
+  match goal with
+    H : age ?x ?y, HH : ?P ?x |- _ =>
+    cut (P y);
+    [ clear HH; intros HH
+    | hered;
+      try apply pred_hered;
+      try apply predicates_hered.exactly_obligation_1]
+  end.
+
+
+(** * Aging and predicates *)
+
+Lemma hereditary_func_at' loc fs :
+  hereditary age (seplog.func_at' fs loc).
+Proof.
+  apply pred_hered.
+Qed.
+
+Lemma anti_hereditary_func_at' loc fs :
+  hereditary (fun x y => age y x) (seplog.func_at' fs loc).
+Proof.
+  intros x y a; destruct fs as [f cc A P Q]; simpl.
+  intros [pp E].
+  destruct (proj2 (age1_PURE _ _ loc (FUN f cc) a)) as [pp' Ey]; eauto.
+  pose proof resource_at_approx y loc as H.
+  rewrite Ey in H at 1; simpl in H.
+  rewrite <-H.
+  exists pp'.
+  reflexivity.
+Qed.
+
+Lemma hereditary_necR {phi phi' : rmap} {P} :
+  necR phi phi' ->
+  hereditary age P ->
+  P phi -> P phi'.
+Proof.
+  intros N H; induction N; auto.
+  apply H; auto.
+Qed.
+
+Lemma anti_hereditary_necR {phi phi' : rmap} {P} :
+  necR phi phi' ->
+  hereditary (fun x y => age y x) P ->
+  P phi' -> P phi.
+Proof.
+  intros N H; induction N; auto.
+  apply H; auto.
+Qed.
+
+Lemma app_pred_age {R} {phi phi' : rmap} :
+  age phi phi' ->
+  app_pred R phi ->
+  app_pred R phi'.
+Proof.
+  destruct R as [R HR]; simpl.
+  apply HR.
+Qed.
+
+Lemma age_yes_sat {Phi Phi' phi phi' l z sh sh'} (R : mpred) :
+  level Phi = level phi ->
+  age Phi Phi' ->
+  age phi phi' ->
+  app_pred R phi ->
+  Phi  @ l = YES sh sh' (LK z) (SomeP nil (fun _ => R)) ->
+  app_pred (approx (S (level phi')) R) phi' /\
+  Phi' @ l = YES sh sh' (LK z) (SomeP nil (fun _ => approx (level Phi') R)).
+Proof.
+  intros L A Au SAT AT.
+  pose proof (app_pred_age Au SAT) as SAT'.
+  split.
+  - split.
+    + apply age_level in A; apply age_level in Au. omega.
+    + apply SAT'.
+  - apply (necR_YES _ Phi') in AT.
+    + rewrite AT.
+      reflexivity.
+    + constructor. assumption.
+Qed.
+
+Lemma age_resource_at {phi phi' loc} :
+  age phi phi' ->
+  phi' @ loc = resource_fmap (approx (level phi')) (phi @ loc).
+Proof.
+  intros A.
+  rewrite <- (age1_resource_at _ _ A loc (phi @ loc)).
+  - reflexivity.
+  - rewrite resource_at_approx. reflexivity.
+Qed.
+
+Lemma age_to_resource_at phi n loc : age_to n phi @ loc = resource_fmap (approx n) (phi @ loc).
+Proof.
+  assert (D : (n <= level phi \/ n >= level phi)%nat) by omega.
+  destruct D as [D | D]; swap 1 2.
+  - rewrite age_to_ge; auto.
+    rewrite <-resource_at_approx.
+    change compcert_rmaps.R.resource_fmap with resource_fmap.
+    change compcert_rmaps.R.approx with approx.
+    match goal with
+      |- _ = ?map ?f (?map ?g ?r) => transitivity (map (f oo g) r)
+    end; swap 1 2.
+    + destruct (phi @ loc); unfold "oo"; simpl; auto.
+      * destruct p0; auto.
+      * destruct p; auto.
+    + f_equal. rewrite approx_oo_approx''; auto.
+  - generalize (age_to_ageN n phi).
+    generalize (age_to n phi); intros phi'.
+    replace n with (level phi - (level phi - n))%nat at 2 by omega.
+    generalize (level phi - n)%nat; intros k. clear n D.
+    revert phi phi'; induction k; intros phi phi'.
+    + unfold ageN in *; simpl.
+      injection 1 as <-.
+      simpl; replace (level phi - 0)%nat with (level phi) by omega.
+      symmetry.
+      apply resource_at_approx.
+    + change (ageN (S k) phi) with
+      (match age1 phi with Some w' => ageN k w' | None => None end).
+      destruct (age1 phi) as [o|] eqn:Eo. 2:congruence.
+      intros A; specialize (IHk _ _ A).
+      rewrite IHk.
+      pose proof age_resource_at Eo (loc := loc) as R.
+      rewrite R.
+      clear A R.
+      rewrite (age_level _ _ Eo).
+      simpl.
+      match goal with
+        |- ?map ?f (?map ?g ?r) = _ => transitivity (map (f oo g) r)
+      end.
+      * destruct (phi @ loc); unfold "oo"; simpl; auto.
+        -- destruct p0; auto.
+        -- destruct p; auto.
+      * f_equal. rewrite approx_oo_approx'; auto.
+        omega.
+Qed.
+
+Lemma pures_eq_unage {jm1 jm1' jm2}:
+  ge (level jm1') (level jm2) ->
+  age jm1 jm1' ->
+  juicy_safety.pures_eq jm1' jm2 ->
+  juicy_safety.pures_eq jm1 jm2.
+Proof.
+  intros L A [S P]; split; intros loc; [clear P; autospec S | clear S; autospec P ].
+  all:apply age_jm_phi in A.
+  all:repeat rewrite level_juice_level_phi in *.
+  all:unfold m_phi in *.
+  all:destruct jm1 as [_ p1 _ _ _ _].
+  all:destruct jm1' as [_ p1' _ _ _ _].
+  all:destruct jm2 as [_ p2 _ _ _ _].
+  - rewrite (age_resource_at A) in S.
+    destruct (p1 @ loc) eqn:E; auto.
+    simpl in S.
+    rewrite S.
+    rewrite preds_fmap_fmap.
+    rewrite approx_oo_approx'; auto.
+  
+  - destruct (p2 @ loc) eqn:E; auto.
+    revert P.
+    eapply age1_PURE. auto.
+Qed.
+
+(** * Aging and operational steps *)
+
+Lemma jstep_age_sim {G C} {csem : CoreSemantics G C mem} {ge c c' jm1 jm2 jm1'} :
+  age jm1 jm2 ->
+  jstep csem ge c jm1 c' jm1' ->
+  level jm2 <> O ->
+  exists jm2',
+    age jm1' jm2' /\
+    jstep csem ge c jm2 c' jm2'.
+Proof.
+  intros A [step [rd lev]] nz.
+  destruct (age1 jm1') as [jm2'|] eqn:E.
+  - exists jm2'. split; auto.
+    split; [|split]; auto.
+    + exact_eq step.
+      f_equal; apply age_jm_dry; auto.
+    + eapply (age_resource_decay _ (m_phi jm1) (m_phi jm1')).
+      * exact_eq rd.
+        f_equal. f_equal. apply age_jm_dry; auto.
+      * apply age_jm_phi; auto.
+      * apply age_jm_phi; auto.
+      * rewrite level_juice_level_phi in *. auto.
+    + apply age_level in E.
+      apply age_level in A.
+      omega.
+  - apply age1_level0 in E.
+    apply age_level in A.
+    omega.
+Qed.
+
+Lemma jsafeN_age Z Jspec ge ora q n jm jmaged :
+  ext_spec_stable age (JE_spec _ Jspec) ->
+  age jm jmaged ->
+  le n (level jmaged) ->
+  @jsafeN Z Jspec ge n ora q jm ->
+  @jsafeN Z Jspec ge n ora q jmaged.
+Proof.
+  intros heredspec A L Safe; revert jmaged A L.
+  induction Safe as
+      [ z c jm
+      | n z c jm c' jm' step safe IH
+      | n z c jm ef sig args x atex Pre Post
+      | n z c jm v Halt Exit ]; intros jmaged A L.
+  - constructor 1.
+  - simpl in step.
+    destruct (jstep_age_sim A step ltac:(omega)) as [jmaged' [A' step']].
+    econstructor 2; eauto.
+    apply IH; eauto.
+    apply age_level in A'.
+    apply age_level in A.
+    destruct step as [_ [_ ?]].
+    omega.
+  - econstructor 3.
+    + eauto.
+    + eapply (proj1 heredspec); eauto.
+    + intros ret jm' z' n' H rel post.
+      destruct (Post ret jm' z' n' H) as (c' & atex' & safe'); eauto.
+      unfold juicy_safety.Hrel in *.
+      split;[|split]; try apply rel.
+      * apply age_level in A; omega.
+      * unshelve eapply (pures_eq_unage _ A), rel.
+        omega.
+  - econstructor 4. eauto.
+    eapply (proj2 heredspec); eauto.
+Qed.
+
+
+Lemma jsafeN_age_to Z Jspec ge ora q n l jm :
+  ext_spec_stable age (JE_spec _ Jspec) ->
+  le n l ->
+  @jsafeN Z Jspec ge n ora q jm ->
+  @jsafeN Z Jspec ge n ora q (age_to l jm).
+Proof.
+  intros Stable nl.
+  apply age_to_ind_refined.
+  intros x y H L.
+  apply jsafeN_age; auto.
+  omega.
+Qed.
+
+Lemma m_dry_age_to n jm : m_dry (age_to n jm) = m_dry jm.
+Proof.
+  remember (m_dry jm) as m eqn:E; symmetry; revert E.
+  apply age_to_ind; auto.
+  intros x y H E ->. rewrite E; auto. clear E.
+  apply age_jm_dry; auto.
+Qed.
+
+Lemma m_phi_age_to n jm : m_phi (age_to n jm) = age_to n (m_phi jm).
+Proof.
+  unfold age_to.
+  rewrite level_juice_level_phi.
+  generalize (level (m_phi jm) - n)%nat; clear n.
+  intros n; induction n. reflexivity.
+  simpl. rewrite <- IHn.
+  clear IHn. generalize (age_by n jm); clear jm; intros jm.
+  unfold age1'.
+  destruct (age1 jm) as [jm'|] eqn:e.
+  - rewrite (age1_juicy_mem_Some _ _ e). easy.
+  - rewrite (age1_juicy_mem_None1 _ e). easy.
+Qed.
