concurrency/semax_to_safety.v
@@ -1,0 +1,337 @@
+Require Import Coq.Strings.String.
+
+Require Import compcert.lib.Integers.
+Require Import compcert.common.AST.
+Require Import compcert.cfrontend.Clight.
+Require Import compcert.common.Globalenvs.
+Require Import compcert.common.Memory.
+Require Import compcert.common.Memdata.
+Require Import compcert.common.Values.
+
+Require Import msl.Coqlib2.
+Require Import msl.eq_dec.
+Require Import msl.seplog.
+Require Import veric.initial_world.
+Require Import veric.juicy_mem.
+Require Import veric.juicy_mem_lemmas.
+Require Import veric.semax_prog.
+Require Import veric.compcert_rmaps.
+Require Import veric.Clight_new.
+Require Import veric.Clightnew_coop.
+Require Import veric.semax.
+Require Import veric.semax_ext.
+Require Import veric.juicy_extspec.
+Require Import veric.initial_world.
+Require Import veric.juicy_extspec.
+Require Import veric.tycontext.
+Require Import veric.semax_ext.
+Require Import veric.semax_ext_oracle.
+Require Import veric.res_predicates.
+Require Import veric.mem_lessdef.
+Require Import floyd.coqlib3.
+Require Import sepcomp.semantics.
+Require Import sepcomp.step_lemmas.
+Require Import sepcomp.event_semantics.
+Require Import concurrency.coqlib5.
+Require Import concurrency.semax_conc.
+Require Import concurrency.juicy_machine.
+Require Import concurrency.concurrent_machine.
+Require Import concurrency.scheduler.
+Require Import concurrency.addressFiniteMap.
+Require Import concurrency.permissions.
+Require Import concurrency.JuicyMachineModule.
+Require Import concurrency.age_to.
+Require Import concurrency.sync_preds_defs.
+Require Import concurrency.sync_preds.
+Require Import concurrency.join_lemmas.
+Require Import concurrency.aging_lemmas.
+Require Import concurrency.cl_step_lemmas.
+Require Import concurrency.resource_decay_lemmas.
+Require Import concurrency.resource_decay_join.
+Require Import concurrency.semax_invariant.
+Require Import concurrency.sync_preds.
+Require Import concurrency.semax_invariant.
+Require Import concurrency.semax_initial.
+Require Import concurrency.semax_progress.
+Require Import concurrency.semax_to_juicy_machine.
+
+Inductive jmsafe : nat -> cm_state -> Prop :=
+| jmsafe_0 m ge sch tp : jmsafe 0 (m, ge, (sch, tp))
+| jmsafe_halted n m ge tp : jmsafe n (m, ge, (nil, tp))
+| jmsafe_core n m m' ge sch tp tp':
+    @JuicyMachine.machine_step ge sch nil tp m sch nil tp' m' ->
+    jmsafe n (m', ge, (sch, tp')) ->
+    jmsafe (S n) (m, ge, (sch, tp))
+| jmsafe_sch n m m' ge i sch tp tp':
+    @JuicyMachine.machine_step ge (i :: sch) nil tp m sch nil tp' m' ->
+    (forall sch', jmsafe n (m', ge, (sch', tp'))) ->
+    jmsafe (S n) (m, ge, (i :: sch, tp)).
+
+(*
+Inductive jmsafe : nat -> cm_state -> Prop :=
+| jmsafe_0 m ge sch tp : jmsafe 0 (m, ge, (sch, tp))
+| jmsafe_halted n m ge tp : jmsafe n (m, ge, (nil, tp))
+| jmsafe_sch n m m' ge i sch tp tp':
+    @JuicyMachine.machine_step ge (i :: sch) nil tp m sch nil tp' m' ->
+    (forall sch', unique_Krun tp sch' -> jmsafe n (m', ge, (sch', tp'))) ->
+    jmsafe (S n) (m, ge, (i :: sch, tp)).
+ *)
+
+Lemma step_sch_irr ge i sch sch' tp m tp' m' :
+  @JuicyMachine.machine_step ge (i :: sch) nil tp m sch nil tp' m' ->
+  @JuicyMachine.machine_step ge (i :: sch') nil tp m sch' nil tp' m'.
+Proof.
+  intros step.
+  assert (i :: sch <> sch) by (clear; induction sch; congruence).
+  inversion step; try solve [exfalso; eauto].
+  - now eapply JuicyMachine.suspend_step; eauto.
+  - now eapply JuicyMachine.sync_step; eauto.
+  - now eapply JuicyMachine.halted_step; eauto.
+  - now eapply JuicyMachine.schedfail; eauto.
+Qed.
+
+(*+ Final instantiation *)
+
+Section Safety.
+  Variables
+    (CS : compspecs)
+    (V : varspecs)
+    (G : funspecs)
+    (ext_link : string -> ident)
+    (ext_link_inj : forall s1 s2, ext_link s1 = ext_link s2 -> s1 = s2)
+    (prog : Clight.program)
+    (all_safe : semax_prog.semax_prog (Concurrent_Espec unit CS ext_link) prog V G)
+    (init_mem_not_none : Genv.init_mem prog <> None).
+  
+  Definition Jspec' := (@OK_spec (Concurrent_Espec unit CS ext_link)).
+  
+  (* another, looser invariant to have more standard preservation
+  statement *)
+  Definition inv Gamma n state :=
+    exists m, n <= m /\ state_invariant Jspec' Gamma m state.
+
+  Lemma inv_sch_irr Gamma n m ge i sch sch' tp :
+    inv Gamma n (m, ge, (i :: sch, tp)) ->
+    inv Gamma n (m, ge, (i :: sch', tp)).
+  Proof.
+    intros (k & lkm & Hk).
+    exists k; split; auto.
+    eapply state_invariant_sch_irr, Hk.
+  Qed.
+  
+  Lemma state_invariant_step Gamma n state :
+    state_invariant Jspec' Gamma (S n) state ->
+    exists state',
+      state_step state state' /\
+      (state_invariant Jspec' Gamma n state' \/
+       state_invariant Jspec' Gamma (S n) state').
+  Proof.
+    intros inv.
+    destruct (progress CS ext_link ext_link_inj _ _ _ inv) as (state', step).
+    exists state'; split; [ now apply step | ].
+    eapply preservation; eauto.
+  Qed.
+  
+  Theorem progress_inv Gamma n state :
+    inv Gamma (S n) state -> exists state', state_step state state'.
+  Proof.
+    intros (m & lm & i).
+    replace m with (S (m - 1)) in i by omega.
+    apply (progress CS ext_link ext_link_inj _ _ _ i).
+  Qed.
+  
+  Theorem preservation_inv Gamma n state state' :
+    state_step state state' -> inv Gamma (S n) state -> inv Gamma n state'.
+  Proof.
+    unfold inv; intros s (m & lm & i).
+    replace m with (S (m - 1)) in i by omega.
+    destruct (preservation CS ext_link ext_link_inj _ _ _ _ s i) as [H|H].
+    - exists (m - 1). split. omega. assumption.
+    - exists m. split. omega. exact_eq H; f_equal. omega.
+  Qed.
+  
+  Lemma inv_step Gamma n state :
+    inv Gamma (S n) state ->
+    exists state',
+      state_step state state' /\
+      inv Gamma n state'.
+  Proof.
+    intros inv.
+    destruct (progress_inv _ _ _ inv) as (state', step).
+    exists state'; split; [ now apply step | ].
+    eapply preservation_inv; eauto.
+  Qed.
+  
+  Lemma invariant_safe Gamma n state :
+    inv Gamma n state -> jmsafe n state.
+  Proof.
+    intros INV.
+    pose proof (progress_inv) as Progress.
+    pose proof (preservation_inv) as Preservation.
+    revert state INV.
+    induction n; intros ((m, ge), (sch, tp)) INV.
+    - apply jmsafe_0.
+    - destruct sch.
+      + apply jmsafe_halted.
+      + destruct (Progress _ _ _ INV) as (state', step).
+        pose proof (Preservation _ _ _ _ step INV).
+        inversion step as [ | ge' m0 m' sch' sch'' tp0 tp' jmstep ]; subst; simpl in *.
+        inversion jmstep; subst.
+        * eapply jmsafe_core; eauto.
+        * eapply jmsafe_core; eauto.
+        * eapply jmsafe_core; eauto.
+        * eapply jmsafe_sch; eauto.
+          intros sch'; apply IHn.
+          eapply (step_sch_irr _ _ _ sch') in jmstep.
+          simpl in *.
+          assert (step' : state_step (m', ge, (t0 :: sch', tp)) (m', ge, (sch', tp'))).
+          { constructor; auto. }
+          eapply inv_sch_irr in INV.
+          specialize (Preservation _ _ _ _ step' INV).
+          assumption.
+        * eapply jmsafe_sch; eauto.
+          intros sch'; apply IHn.
+          eapply (step_sch_irr _ _ _ sch') in jmstep.
+          simpl in *.
+          assert (step' : state_step (m, ge, (t0 :: sch', tp)) (m', ge, (sch', tp'))).
+          { constructor; auto. }
+          eapply inv_sch_irr in INV.
+          specialize (Preservation _ _ _ _ step' INV).
+          assumption.
+        * eapply jmsafe_sch; eauto.
+          intros sch'; apply IHn.
+          eapply (step_sch_irr _ _ _ sch') in jmstep.
+          simpl in *.
+          assert (step' : state_step (m', ge, (t0 :: sch', tp')) (m', ge, (sch', tp'))).
+          { constructor; auto. }
+          eapply inv_sch_irr in INV.
+          specialize (Preservation _ _ _ _ step' INV).
+          assumption.
+        * eapply jmsafe_sch; eauto.
+          intros sch'; apply IHn.
+          eapply (step_sch_irr _ _ _ sch') in jmstep.
+          simpl in *.
+          assert (step' : state_step (m', ge, (t0 :: sch', tp')) (m', ge, (sch', tp'))).
+          { constructor; auto. }
+          eapply inv_sch_irr in INV.
+          specialize (Preservation _ _ _ _ step' INV).
+          assumption.
+  Qed.
+  
+  Definition init_mem : { m | Genv.init_mem prog = Some m } := init_m prog init_mem_not_none.
+  
+  Definition spr :=
+    semax_prog_rule
+      (Concurrent_Espec unit CS ext_link) V G prog
+      (proj1_sig init_mem) all_safe (proj2_sig init_mem).
+  
+  Definition initial_corestate : corestate := projT1 (projT2 spr).
+  
+  Definition initial_jm (n : nat) : juicy_mem := proj1_sig (snd (projT2 (projT2 spr)) n).
+  
+  Definition initial_machine_state (n : nat) :=
+    ThreadPool.mk
+      (pos.mkPos (le_n 1))
+      (fun _ => Krun initial_corestate)
+      (fun _ => m_phi (initial_jm n))
+      (addressFiniteMap.AMap.empty _).
+
+  Definition NoExternal_Espec : external_specification mem external_function unit :=
+    Build_external_specification
+      _ _ _
+      (* no external calls from the machine *)
+      (fun _ => False)
+      (fun _ _ _ _ _ _ _ => False)
+      (fun _ _ _ _ _ _ _ => False)
+      (* when the machine is halted, it means no more schedule, there
+      is nothing to check: *)
+      (fun _ _ _ => Logic.True).
+  
+  Definition NoExternal_Hrel : nat -> mem -> mem -> Prop := fun _ _ _ => False.
+  
+  (* We state the theorem in terms of [safeN_] but because there are
+  no external, this really just says that the initial state is
+  "angelically safe" : for every schedule and every fuel n, there is a
+  path either ending on an empty schedule or consuming all the
+  fuel. *)
+  
+  Theorem safe_initial_state : forall sch r n genv_symb,
+      safeN_
+        (G := genv)
+        (C := schedule * list _ * ThreadPool.t)
+        (M := mem)
+        (Z := unit)
+        (genv_symb := genv_symb)
+        (Hrel := NoExternal_Hrel)
+        (JuicyMachine.MachineSemantics sch r)
+        NoExternal_Espec
+        (globalenv prog)
+        n
+        tt
+        (sch, nil, initial_machine_state n)
+        (proj1_sig init_mem).
+  Proof.
+    intros sch r n thisfunction.
+    pose proof initial_invariant CS V G ext_link prog as INIT.
+    repeat (specialize (INIT ltac:(assumption))).
+    match type of INIT with
+      _ _ ?a n ?b =>
+      assert (init : inv a n b) by (hnf; eauto)
+    end.
+    pose proof inv_step as SIM.
+    clear INIT; revert init.
+    unfold initial_state, initial_machine_state.
+    unfold initial_corestate, initial_jm, spr, init_mem.
+    match goal with |- context[(sch, ?tp)] => generalize tp end.
+    match goal with |- context[(proj1_sig ?m)] => generalize (proj1_sig m) end.
+    (* here we decorelate the CoreSemantics parameters from the
+    initial state parameters *)
+    generalize sch at 2.
+    generalize (globalenv prog), sch.
+    clear -SIM.
+    induction n; intros g sch schSEM m t INV; [ now constructor | ].
+    destruct (SIM _ _ _ INV) as [cm' [step INV']].
+    inversion step as [ | ? ? m' ? sch' ? tp' STEP ]; subst; clear step.
+    - (* empty schedule *)
+      eapply safeN_halted.
+      + reflexivity.
+      + apply I.
+    - (* a step can be taken *)
+      eapply safeN_step with (c' := (sch', nil, tp')) (m'0 := m').
+      + eapply STEP.
+      + apply IHn.
+        apply INV'.
+  Qed.
+  
+  (* The following is a slightly stronger result, proving [jmsafe]
+  i.e. a safety that universally quantifies over all schedule each
+  time a part of the schedule is consumed *)
+
+  Theorem jmsafe_initial_state sch n :
+    jmsafe n ((proj1_sig init_mem, globalenv prog), (sch, initial_machine_state n)).
+  Proof.
+    eapply invariant_safe.
+    exists n; split; auto; apply initial_invariant.
+  Qed.
+  
+  Lemma jmsafe_csafe n m ge sch s : jmsafe n (m, ge, (sch, s)) -> JuicyMachine.csafe ge (sch, nil, s) m n.
+  Proof.
+    clear.
+    revert m ge sch s; induction n; intros m ge sch s SAFE.
+    now constructor 1.
+    inversion SAFE; subst.
+    - constructor 2. reflexivity.
+    - econstructor 3; simpl; eauto.
+    - econstructor 4; simpl; eauto.
+  Qed.
+  
+  (* [jmsafe] is an intermediate result, we can probably prove [csafe]
+  directly *)
+  
+  Theorem safety_initial_state (sch : schedule) (n : nat) :
+    JuicyMachine.csafe (globalenv prog) (sch, nil, initial_machine_state n) (proj1_sig init_mem) n.
+  Proof.
+    apply jmsafe_csafe, jmsafe_initial_state.
+  Qed.
+  
+End Safety.
