concurrency/sync_preds_defs.v
@@ -1,0 +1,134 @@
+Require Import msl.Coqlib2.
+Require Import msl.eq_dec.
+Require Import msl.seplog.
+Require Import veric.compcert_rmaps.
+Require Import veric.tycontext.
+Require Import veric.res_predicates.
+Require Import concurrency.addressFiniteMap.
+
+Set Bullet Behavior "Strict Subproofs".
+
+(* Those were overwritten in structured_injections *)
+Notation join := sepalg.join.
+Notation join_assoc := sepalg.join_assoc.
+
+Definition islock_pred R r := exists sh sh' z, r = YES sh sh' (LK z) (SomeP nil (fun _ => R)).
+
+Lemma islock_pred_join_sub {r1 r2 R} : join_sub r1 r2 -> islock_pred R r1  -> islock_pred R r2.
+Proof.
+  intros [r0 J] [x [sh' [z ->]]].
+  inversion J; subst; eexists; eauto.
+Qed.
+
+Definition LKspec_ext (R: pred rmap) : spec :=
+   fun (rsh sh: Share.t) (l: AV.address)  =>
+    allp (jam (adr_range_dec l lock_size)
+                         (jam (eq_dec l) 
+                            (yesat (SomeP nil (fun _ => R)) (LK lock_size) rsh sh)
+                            (CTat l rsh sh))
+                         (fun _ => TT)).
+
+Definition LK_at R sh :=
+  LKspec_ext R (Share.unrel Share.Lsh sh) (Share.unrel Share.Rsh sh).
+
+Definition isLK (r : resource) := exists sh sh' z P, r = YES sh sh' (LK z) P.
+
+Definition isCT (r : resource) := exists sh sh' z P, r = YES sh sh' (CT z) P.
+
+Definition resource_is_lock r := exists rsh sh n pp, r = YES rsh sh (LK n) pp.
+
+Definition same_locks phi1 phi2 := 
+  forall loc, resource_is_lock (phi1 @ loc) <-> resource_is_lock (phi2 @ loc).
+
+Definition resource_is_lock_sized n r := exists rsh sh pp, r = YES rsh sh (LK n) pp.
+
+Definition same_locks_sized phi1 phi2 := 
+  forall loc n, resource_is_lock_sized n (phi1 @ loc) <-> resource_is_lock_sized n (phi2 @ loc).
+
+Definition lockSet_block_bound lset b :=
+  forall loc, isSome (AMap.find (elt:=option rmap) loc lset) -> (fst loc < b)%positive.
+
+Definition predat phi loc R :=
+  exists sh sh' z, phi @ loc = YES sh sh' (LK z) (SomeP nil (fun _ => R)).
+
+Definition rmap_bound b phi :=
+  (forall loc, (fst loc >= b)%positive -> phi @ loc = NO Share.bot).
+
+(* Constructive version of resource_decay (equivalent to the
+non-constructive version, see resource_decay_join.v) *)
+Definition resource_decay_aux (nextb: block) (phi1 phi2: rmap) : Type :=
+  prod (level phi1 >= level phi2)%nat
+  (forall l: address,
+    
+  ((fst l >= nextb)%positive -> phi1 @ l = NO Share.bot) *
+  ( (resource_fmap (approx (level phi2)) (phi1 @ l) = (phi2 @ l))
+    
+  + { rsh : _ & { v : _ & { v' : _ |
+       resource_fmap (approx (level phi2)) (phi1 @ l) = YES rsh pfullshare (VAL v) NoneP /\ 
+       phi2 @ l = YES rsh pfullshare (VAL v') NoneP }}}
+  
+  + (fst l >= nextb)%positive * { v | phi2 @ l = YES Share.top pfullshare (VAL v) NoneP }
+  
+  + { v : _ & { pp : _ | phi1 @ l = YES Share.top pfullshare (VAL v) pp /\ phi2 @ l = NO Share.bot } })).
+
+Ltac breakhyps :=
+  repeat
+    match goal with
+      H : _ \/ _  |- _ => destruct H
+    | H : _ /\ _  |- _ => destruct H
+    | H : prod _ _  |- _ => destruct H
+    | H : sum _ _  |- _ => destruct H
+    | H : sumbool _ _  |- _ => destruct H
+    | H : sumor _ _  |- _ => destruct H
+    | H : ex _  |- _ => destruct H
+    | H : sig _  |- _ => destruct H
+    | H : sigT _  |- _ => destruct H
+    | H : sigT2 _  |- _ => destruct H
+    end;
+  discriminate || congruence || tauto || auto.
+
+Ltac check_false P :=
+  let F := fresh "false" in
+  assert (F : P -> False) by (intro; breakhyps);
+  clear F.
+
+Ltac sumsimpl :=
+  match goal with
+    |- sum ?A ?B => check_false A; right
+  | |- sum ?A ?B => check_false B; left
+  | |- sumor ?A ?B => check_false A; right
+  | |- sumor ?A ?B => check_false B; left
+  | |- sumbool ?A ?B => check_false A; right
+  | |- sumbool ?A ?B => check_false B; left
+  end.
+
+Definition resource_decay_at (nextb: block) n (r1 r2 : resource) b := 
+  ((b >= nextb)%positive -> r1 = NO Share.bot) /\
+  (resource_fmap (approx (n)) (r1) = (r2) \/
+  (exists rsh, exists v, exists v',
+       resource_fmap (approx (n)) (r1) = YES rsh pfullshare (VAL v) NoneP /\ 
+       r2 = YES rsh pfullshare (VAL v') NoneP)
+  \/ ((b >= nextb)%positive /\ exists v, r2 = YES Share.top pfullshare (VAL v) NoneP)
+  \/ (exists v, exists pp, r1 = YES Share.top pfullshare (VAL v) pp /\ r2 = NO Share.bot)).
+
+Ltac range_tac :=
+  match goal with
+  | H : ~ adr_range (?b, _) _ (?b, _) |- _ =>
+    exfalso; apply H;
+    repeat split; auto;
+    try unfold Int.unsigned;
+    unfold lock_size;
+    omega
+  | H : ~ adr_range ?l _ ?l |- _ =>
+    destruct l;
+    exfalso; apply H;
+    repeat split; auto;
+    try unfold Int.unsigned;
+    unfold lock_size;
+    omega
+  end.
+
+Ltac eassert :=
+  let mp := fresh "mp" in
+  pose (mp := fun {goal Q : Type} (x : goal) (y : goal -> Q) => y x);
+  eapply mp; clear mp.
